specs/Spec.Blake2s.fst
@@ -197,18 +197,15 @@ let blake2s_internal2 dd d h =
   else h
 
 
-val blake2s_internal3 : h:intseq U32 8 -> dd:size_nat{0 < dd /\ dd * bytes_in_block <= max_size_t} -> d:lbytes (dd * bytes_in_block) -> ll:size_nat -> kk:size_nat{kk<=32} -> nn:size_nat{1 <= nn /\ nn <= 32} -> Tot (lbytes nn)
+val blake2s_internal3 : h:intseq U32 8 -> dd:size_nat{0 < dd /\ dd * bytes_in_block <= max_size_t} -> d:lbytes (dd * bytes_in_block) -> ll:size_nat -> kk:size_nat{kk<=32} -> nn:size_nat{1 <= nn /\ nn <= 32} -> Tot hash_state
 
 let blake2s_internal3 h dd d ll kk nn =
   let offset : size_nat = (dd - 1) * 16 * 4 in
   let last_block : intseq U32 16 = uints_from_bytes_le (sub d offset bytes_in_block) in
-  let h =
-    if kk = 0 then
-      blake2_compress h last_block (u64  ll) true
-    else
-      blake2_compress h last_block (u64 (ll + block_bytes)) true
-  in
-  sub (uints_to_bytes_le h) 0 nn
+  if kk = 0 then
+    blake2_compress h last_block (u64  ll) true
+  else
+    blake2_compress h last_block (u64 (ll + block_bytes)) true
 
 
 val blake2s_internal : dd:size_nat{0 < dd /\ dd * bytes_in_block <= max_size_t} -> d:lbytes (dd * bytes_in_block) -> ll:size_nat -> kk:size_nat{kk<=32} -> nn:size_nat{1 <= nn /\ nn <= 32} -> Tot (lbytes nn)
@@ -216,8 +213,9 @@ let blake2s_internal dd d ll kk nn =
   let h = const_init in
   let h = blake2s_internal1 h kk nn in
   let h = blake2s_internal2 dd d h in
-  let k = blake2s_internal3 h dd d ll kk nn in
-  k
+  let h = blake2s_internal3 h dd d ll kk nn in
+  sub (uints_to_bytes_le h) 0 nn
+
 
 val blake2s : ll:size_nat{0 < ll /\ ll <= max_size_t - 2 * bytes_in_block } ->  d:lbytes ll ->  kk:size_nat{kk<=32} -> k:lbytes kk -> nn:size_nat{1 <= nn /\ nn <= 32} -> Tot (lbytes nn)
 
